Unsigned.thy
@@ -1,57 +1,139 @@
 theory Unsigned
-  imports Main HOL.Nat
+  imports Main HOL.Nat "HOL-Library.Monad_Syntax"
 begin
 
 datatype u8 = u8 nat
 datatype u64 = u64 nat
+datatype Slot = Slot u64
+datatype Epoch = Epoch u64
 
 primrec u64_to_nat :: "u64 \<Rightarrow> nat" where
   "u64_to_nat (u64 n) = n"
 
+primrec slot_to_u64 :: "Slot \<Rightarrow> u64" where
+  "slot_to_u64 (Slot n) = n"
+
+primrec epoch_to_u64 :: "Epoch \<Rightarrow> u64" where
+  "epoch_to_u64 (Epoch n) = n"
+
 definition valid_u64 :: "u64 \<Rightarrow> bool" where
   "valid_u64 n \<equiv> u64_to_nat n < 2 ^ 64"
+
+definition valid_slot :: "Slot \<Rightarrow> bool" where
+  "valid_slot s \<equiv> valid_u64 (slot_to_u64 s)"
+
+definition valid_epoch :: "Epoch \<Rightarrow> bool" where
+  "valid_epoch e \<equiv> valid_u64 (epoch_to_u64 e)"
+
+consts
+  unsigned_add :: "'a \<Rightarrow> 'a \<Rightarrow> 'a option"
+  unsigned_sub :: "'a \<Rightarrow> 'a \<Rightarrow> 'a option"
+  unsigned_mul :: "'a \<Rightarrow> 'a \<Rightarrow> 'a option"
+  unsigned_div :: "'a \<Rightarrow> 'a \<Rightarrow> 'a option"
+
+notation
+  unsigned_add (infixl ".+" 65) and
+  unsigned_sub (infixl ".-" 65) and
+  unsigned_mul (infixl ".*" 70) and
+  unsigned_div (infixl "\\" 70)
+
+definition check_bin_op_then ::
+  "('a \<Rightarrow> 'b) \<Rightarrow>
+   ('b \<Rightarrow> 'a) \<Rightarrow>
+   ('a \<Rightarrow> 'a \<Rightarrow> bool) \<Rightarrow>
+   ('a \<Rightarrow> bool) \<Rightarrow>
+   ('b \<Rightarrow> 'b \<Rightarrow> 'b option) \<Rightarrow>
+   'a \<Rightarrow> 'a \<Rightarrow> 'a option" where
+  "check_bin_op_then unwrap wrap arg_check check op x y \<equiv>
+    if arg_check x y then do {
+      result_b \<leftarrow> op (unwrap x) (unwrap y);
+      let result_a = wrap result_b;
+      if check result_a then Some result_a else None
+    } else None"
 
 definition check_bin_op ::
   "('a \<Rightarrow> 'b) \<Rightarrow>
    ('b \<Rightarrow> 'a) \<Rightarrow>
+   ('a \<Rightarrow> 'a \<Rightarrow> bool) \<Rightarrow>
    ('a \<Rightarrow> bool) \<Rightarrow>
    ('b \<Rightarrow> 'b \<Rightarrow> 'b) \<Rightarrow>
    'a \<Rightarrow> 'a \<Rightarrow> 'a option" where
-  "check_bin_op unwrap wrap check op x y \<equiv>
-    let result = wrap (op (unwrap x) (unwrap y)) in
-    if check result then Some result else None"
+  "check_bin_op unwrap wrap arg_check check op \<equiv>
+    check_bin_op_then unwrap wrap arg_check check (\<lambda>x y. Some (op x y))"
 
-definition u64_add :: "u64 \<Rightarrow> u64 \<Rightarrow> u64 option" (infixl ".+" 65) where
-  "u64_add x y \<equiv> check_bin_op u64_to_nat u64 valid_u64 (+) x y"
+definition any_args :: "'a \<Rightarrow> 'a \<Rightarrow> bool" where
+  "any_args _ _ \<equiv> True"
 
-definition u64_sub :: "u64 \<Rightarrow> u64 \<Rightarrow> u64 option" (infixl ".-" 65) where
-  "u64_sub x y \<equiv>
-    if u64_to_nat x \<ge> u64_to_nat y then
-      check_bin_op u64_to_nat u64 valid_u64 (-) x y
-    else
-      None"
+definition u64_add :: "u64 \<Rightarrow> u64 \<Rightarrow> u64 option" where
+  "u64_add \<equiv> check_bin_op u64_to_nat u64 any_args valid_u64 (+)"
 
-definition u64_mul :: "u64 \<Rightarrow> u64 \<Rightarrow> u64 option" (infixl ".*" 70) where
-  "u64_mul x y \<equiv> check_bin_op u64_to_nat u64 valid_u64 (*) x y"
+definition u64_sub :: "u64 \<Rightarrow> u64 \<Rightarrow> u64 option" where
+  "u64_sub \<equiv>
+    check_bin_op u64_to_nat u64 (\<lambda>x y. u64_to_nat x \<ge> u64_to_nat y) valid_u64 (-)"
 
-definition u64_div :: "u64 \<Rightarrow> u64 \<Rightarrow> u64 option" (infixl "\\" 70) where
-  "u64_div x y \<equiv>
-    if y = u64 0 then
-      None
-    else
-      check_bin_op u64_to_nat u64 valid_u64 ((div)) x y"
+definition u64_mul :: "u64 \<Rightarrow> u64 \<Rightarrow> u64 option" where
+  "u64_mul \<equiv> check_bin_op u64_to_nat u64 any_args valid_u64 (*)"
+
+definition u64_div :: "u64 \<Rightarrow> u64 \<Rightarrow> u64 option" where
+  "u64_div \<equiv> check_bin_op u64_to_nat u64 (\<lambda>_ y. y \<noteq> u64 0) valid_u64 (div)"
+
+definition lift_slot_bin_op :: "(u64 \<Rightarrow> u64 \<Rightarrow> u64 option) \<Rightarrow> Slot \<Rightarrow> Slot \<Rightarrow> Slot option" where
+  "lift_slot_bin_op \<equiv> check_bin_op_then slot_to_u64 Slot any_args valid_slot"
+
+definition lift_epoch_bin_op :: "(u64 \<Rightarrow> u64 \<Rightarrow> u64 option) \<Rightarrow> Epoch \<Rightarrow> Epoch \<Rightarrow> Epoch option" where
+  "lift_epoch_bin_op \<equiv> check_bin_op_then epoch_to_u64 Epoch any_args valid_epoch"
+
+definition slot_add :: "Slot \<Rightarrow> Slot \<Rightarrow> Slot option" where
+  "slot_add \<equiv> lift_slot_bin_op u64_add"
+
+definition slot_sub :: "Slot \<Rightarrow> Slot \<Rightarrow> Slot option" where
+  "slot_sub \<equiv> lift_slot_bin_op u64_sub"
+
+definition slot_mul :: "Slot \<Rightarrow> Slot \<Rightarrow> Slot option" where
+  "slot_mul \<equiv> lift_slot_bin_op u64_mul"
+
+definition slot_div :: "Slot \<Rightarrow> Slot \<Rightarrow> Slot option" where
+  "slot_div \<equiv> lift_slot_bin_op u64_div"
+
+definition epoch_add :: "Epoch \<Rightarrow> Epoch \<Rightarrow> Epoch option" where
+  "epoch_add \<equiv> lift_epoch_bin_op u64_add"
+
+definition epoch_sub :: "Epoch \<Rightarrow> Epoch \<Rightarrow> Epoch option" where
+  "epoch_sub \<equiv> lift_epoch_bin_op u64_sub"
+
+definition epoch_mul :: "Epoch \<Rightarrow> Epoch \<Rightarrow> Epoch option" where
+  "epoch_mul \<equiv> lift_epoch_bin_op u64_mul"
+
+definition epoch_div :: "Epoch \<Rightarrow> Epoch \<Rightarrow> Epoch option" where
+  "epoch_div \<equiv> lift_epoch_bin_op u64_div"
+
+adhoc_overloading
+  unsigned_add u64_add slot_add epoch_add and
+  unsigned_sub u64_sub slot_sub epoch_sub and
+  unsigned_mul u64_mul slot_mul epoch_mul and
+  unsigned_div u64_div slot_div epoch_div
+
+lemmas u64_simps = valid_u64_def u64_add_def u64_sub_def u64_mul_def u64_div_def
+lemmas slot_simps = valid_slot_def slot_add_def slot_sub_def slot_mul_def slot_div_def
+                    lift_slot_bin_op_def
+lemmas epoch_simps = valid_epoch_def epoch_add_def epoch_sub_def epoch_mul_def epoch_div_def
+                     lift_epoch_bin_op_def
+lemmas unsigned_simps = any_args_def check_bin_op_then_def check_bin_op_def
 
 (* Sanity check lemmas *)
 lemma u64_add_overflow_int_max: "u64 (2 ^ 64 - 1) .+ u64 1 = None"
-  by (clarsimp simp: u64_add_def valid_u64_def check_bin_op_def)
+  by (clarsimp simp: u64_simps unsigned_simps)
 
 lemma u64_add_overflow_contradiction: "(u64 (2 ^ 64 - 1) .+ u64 1 = Some (u64 0)) \<Longrightarrow> False"
-  by (clarsimp simp: u64_add_def valid_u64_def check_bin_op_def)
+  by (clarsimp simp: u64_simps unsigned_simps)
 
 lemma u64_sub_overflow_zero: "u64 0 .- u64 1 = None"
-  by (clarsimp simp: u64_sub_def valid_u64_def check_bin_op_def)
+  by (clarsimp simp: u64_simps unsigned_simps)
 
 lemma u64_div_zero: "n \\ u64 0 = None"
-  by (clarsimp simp: u64_div_def valid_u64_def check_bin_op_def)
+  by (clarsimp simp: u64_simps unsigned_simps)
+
+lemma slot_div_zero: "n \\ Slot (u64 0) = None"
+  by (clarsimp simp: slot_simps u64_simps unsigned_simps)
 
 end
