Helpers.thy
@@ -1,0 +1,18 @@
+theory Helpers
+  imports Types Config Invariants "HOL-Library.Monad_Syntax"
+begin
+
+definition get_current_epoch :: "Config \<Rightarrow> BeaconState \<Rightarrow> Epoch option" where
+  "get_current_epoch c state \<equiv>
+    map_option Epoch (slot_to_u64 (slot state) \\ SLOTS_PER_EPOCH c)"
+
+definition get_previous_epoch :: "Config \<Rightarrow> BeaconState \<Rightarrow> Epoch option" where
+  "get_previous_epoch c state \<equiv> do {
+    current_epoch \<leftarrow> get_current_epoch c state;
+    if current_epoch = GENESIS_EPOCH then
+      Some GENESIS_EPOCH
+    else
+      current_epoch .- Epoch (u64 1)
+  }"
+
+end
